swapping pointers with generic lenses

examples/refinement/layering/Refinement.Generic.Lens.fst
@@ -38,21 +38,23 @@ type lens 'a 'b = {
 
 let imem inv = m:HS.mem{inv m}
 
-let get_reads_loc #b #inv (loc:B.loc) (get:get_t (imem inv) b) =
+let eloc = Ghost.erased B.loc
+let l (x:eloc) : GTot B.loc = Ghost.reveal x
+let get_reads_loc #b #inv (loc:eloc) (get:get_t (imem inv) b) =
   forall (h0 h1:imem inv) loc'.
-    B.loc_disjoint loc loc' /\
-    B.modifies loc' h0 h1 ==>
+    B.loc_disjoint (l loc) (l loc') /\
+    B.modifies (l loc') h0 h1 ==>
     get h0 == get h1
 
-let put_modifies_loc #b #inv (loc:B.loc) (put:put_t (imem inv) b) =
+let put_modifies_loc #b #inv (loc:eloc) (put:put_t (imem inv) b) =
   forall (h0:imem inv) (v:b).
-    B.modifies loc h0 (put v h0)
+    B.modifies (l loc) h0 (put v h0)
 
-let invariant_reads_loc inv (loc:B.loc) =
+let invariant_reads_loc inv (loc:eloc) =
   forall h0 h1 loc'.
     inv h0 /\
-    B.loc_disjoint loc loc' /\
-    B.modifies loc' h0 h1 ==>
+    B.loc_disjoint (l loc) (l loc') /\
+    B.modifies (l loc') h0 h1 ==>
     inv h1
 
 let ih_lens inv b loc =
@@ -63,203 +65,28 @@ let ih_lens inv b loc =
 
 
 abstract
-let mods fp snap h0 h1 =
-  (B.modifies fp snap h0 ==>
-   B.modifies fp snap h1) /\
-  B.modifies fp h0 h1
+let mods fp snap (h:HS.mem) =
+  B.modifies (l fp) snap h /\
+  FStar.HyperStack.ST.equal_domains snap h
 
-let st_get_t #a #b #fp #inv (x:a) (l:ih_lens (inv x) b fp) =
-  unit ->
-  Stack b
-  (requires inv x)
-  (ensures (fun h0 b h1 ->
-    h0 == h1 /\
-    b == l.get h0))
-
-let st_put_t #a #b (#fp:B.loc) #inv (x:a) (snap:imem (inv x)) (l:ih_lens (inv x) b fp) =
-  v:b ->
-  Stack unit
-  (requires fun h0 ->
-    inv x h0)
-  (ensures (fun h0 _ h1 ->
-    inv x h1 /\
-    mods fp snap h0 h1 /\
-    v == l.get h1))
+let reveal_mods ()
+  : Lemma (forall fp snap h. {:pattern mods fp snap h}
+            mods fp snap h <==>
+            (B.modifies (l fp) snap h /\
+             FStar.HyperStack.ST.equal_domains snap h))
+  = ()
 
 noeq
 type hs_lens 'a 'b = {
-  footprint: B.loc;
+  footprint: eloc;
   invariant: 'a -> HS.mem -> Type0;
   x:'a;
   snapshot:imem (invariant x);
   l:ih_lens (invariant x) 'b footprint;
-  st_get:st_get_t x l;
-  st_put:st_put_t x snapshot l;
   hs_lens_laws: squash (
     invariant_reads_loc (invariant x) footprint
   );
 }
 
-
-let tup2 #a1 #b1 (l1 : hs_lens a1 b1)
-         #a2 #b2 (l2 : hs_lens a2 b2{
-             l1.snapshot == l2.snapshot /\
-             B.all_disjoint [l1.footprint;
-                             l2.footprint;
-                            ]})
-  : GTot (hs_lens (a1 & a2) (b1 & b2))
-  = let fp =
-      B.loc_union_l [l1.footprint;
-                     l2.footprint
-                     ]
-    in
-    let inv (a, b) h : prop =
-      l1.invariant a h /\
-      l2.invariant b h
-    in
-    let x = l1.x, l2.x in
-    let snap : imem (inv x) = l1.snapshot in
-    let get : get_t (imem (inv x)) (b1 & b2) =
-      fun h ->
-        l1.l.get h,
-        l2.l.get h
-      in
-    let put : put_t (imem (inv x)) (b1 & b2) =
-      fun (v1, v2) h ->
-         l2.l.put v2
-        (l1.l.put v1 h)
-    in
-    let l : ih_lens (inv x) (b1 & b2) fp =
-      {
-        get = get;
-        put = put;
-        lens_laws = ()
-      }
-    in
-    let st_get : st_get_t x l =
-      fun () ->
-        let v1 = l1.st_get () in
-        let v2 = l2.st_get () in
-        v1, v2
-    in
-    let st_put : st_put_t x snap l =
-      fun (v1, v2) ->
-        l1.st_put v1;
-        l2.st_put v2
-    in
-    {
-      footprint = fp;
-      invariant = inv;
-      x = x;
-      l = l;
-      snapshot = snap;
-      st_get=st_get;
-      st_put=st_put;
-      hs_lens_laws = ();
-    }
-
-let tup3 #a1 #b1 (l1 : hs_lens a1 b1)
-         #a2 #b2 (l2 : hs_lens a2 b2)
-         #a3 #b3 (l3 : hs_lens a3 b3{
-             l1.snapshot == l2.snapshot /\
-             l2.snapshot == l3.snapshot /\
-             B.all_disjoint [l1.footprint;
-                             l2.footprint;
-                             l3.footprint
-                            ]})
-  : GTot (hs_lens (a1 & a2 & a3) (b1 & b2 & b3))
-  = let fp =
-      B.loc_union_l [l1.footprint;
-                     l2.footprint;
-                     l3.footprint
-                     ]
-    in
-    let inv (a, b, c) h : prop =
-      l1.invariant a h /\
-      l2.invariant b h /\
-      l3.invariant c h
-    in
-    let x = l1.x, l2.x, l3.x in
-    let snap : imem (inv x) = l1.snapshot in
-    let get : get_t (imem (inv x)) (b1 & b2 & b3) =
-      fun h ->
-        l1.l.get h,
-        l2.l.get h,
-        l3.l.get h
-      in
-    let put : put_t (imem (inv x)) (b1 & b2 & b3) =
-      fun (v1, v2, v3) h ->
-         l3.l.put v3
-        (l2.l.put v2
-        (l1.l.put v1 h))
-    in
-    let l : ih_lens (inv x) (b1 & b2 & b3) fp =
-      {
-        get = get;
-        put = put;
-        lens_laws = ()
-      }
-    in
-    let st_get : st_get_t x l =
-      fun () ->
-        let v1 = l1.st_get () in
-        let v2 = l2.st_get () in
-        let v3 = l3.st_get () in
-        v1, v2, v3
-    in
-    let st_put : st_put_t x snap l =
-      fun (v1, v2, v3) ->
-        l1.st_put v1;
-        l2.st_put v2;
-        l3.st_put v3
-    in
-    {
-      footprint = fp;
-      invariant = inv;
-      x = x;
-      l = l;
-      snapshot = snap;
-      st_get=st_get;
-      st_put=st_put;
-      hs_lens_laws = ();
-    }
-
-let ptr_lens (p:B.pointer 'a) (snap:HS.mem{B.live snap p})
-  : GTot (hs_lens (B.pointer 'a) 'a)
-  = let invariant (x:B.pointer 'a) (h:HS.mem) =
-      B.live h x
-    in
-    let fp = B.loc_buffer p in
-    let get : get_t (imem (invariant p)) 'a =
-      fun h -> B.get h p 0
-    in
-    let put : put_t (imem (invariant p)) 'a =
-      fun v h ->
-        let h1 = B.g_upd p 0 v h in
-        B.g_upd_seq_as_seq p (Seq.upd (B.as_seq h p) 0 v) h;
-        h1
-    in
-    assume (get_put get put);
-    assume (put_modifies_loc fp put);
-    let l : ih_lens (invariant p) 'a fp = {
-         get = get;
-         put = put;
-         lens_laws = ()
-      }
-    in
-    let st_get : st_get_t p l =
-      fun () -> B.index p 0ul
-    in
-    let st_put : st_put_t p snap l =
-      fun v -> B.upd p 0ul v
-    in
-    {
-      footprint = fp;
-      invariant = invariant;
-      x = p;
-      snapshot = snap;
-      l = l;
-      st_get = st_get;
-      st_put = st_put;
-      hs_lens_laws = ()
-    }
+let snap (l:hs_lens 'a 'b) (h:imem (l.invariant l.x)) : hs_lens 'a 'b =
+  {l with snapshot = h}
