examples/refinement/layering/Refinement.Generic.Effect.fst
@@ -1,0 +1,63 @@
+module Refinement.Generic.Effect
+(* The goal of this experiment is to define a simple,
+   abstract memory model on top of HyperStack.
+*)
+open FStar.HyperStack.ST
+module B = LowStar.Buffer
+module HS = FStar.HyperStack
+module HST = FStar.HyperStack.ST
+open Refinement.Generic.Lens
+
+let inv #roots #view (l:hs_lens roots view) (h:HS.mem) =
+  l.invariant l.x h
+
+let mods #roots #view (l:hs_lens roots view) (h:HS.mem) =
+  mods l.footprint l.snapshot h
+
+let get #roots #view (l:hs_lens roots view) (h:HS.mem{inv l h}) =
+  l.l.get h
+
+/// The main computation type provided by this module
+///   `RST a r pre post`
+///    An abstract computation on pairs layered on top of HyperStack.STATE
+effect RST (a:Type)
+           (#roots:Type0)
+           (#view:Type0)
+           (l:hs_lens roots view)
+           (pre: view -> Type)
+           (post: view -> a -> view -> Type) =
+       STATE a
+            (fun (k:a -> HS.mem -> Type)
+               (h0:HS.mem) ->
+               inv l h0 /\
+               pre (get l h0) /\
+               mods l h0 /\
+               (forall (x:a) (h1:HS.mem).
+                 inv l h1 /\             //final memory is also in the invariant
+                 mods l h1 /\
+                 post (get l h0)                //and the user-provided post on pairs
+                      x
+                      (get l h1) ==>
+                k x h1))                        //prove the continuation under this hypothesis
+
+let reader_t
+      #roots
+      #view
+      (l:hs_lens roots view) =
+  s:imem (l.invariant l.x) ->
+  RST view (snap l s)
+  (requires fun _ -> True)
+  (ensures fun v0 v v1 ->
+    v0 == v /\
+    v == v1)
+
+let writer_t
+      #roots
+      #view
+      (l:hs_lens roots view) =
+  s:imem (l.invariant l.x) ->
+  v:view ->
+  RST unit (snap l s)
+  (requires fun _ -> True)
+  (ensures fun _ _ v1 ->
+    v1 == v)
